Runtime/Interface.lean
@@ -2,6 +2,13 @@ import Runtime.Utilities
 
 namespace Interface
 
+/--
+An interface scheme captures the type signature of a dependent map. Specifically, a scheme
+`{ vars, type }` describes the type `(var : vars) → (type var)`.
+
+This type is used to describe the structures of components in reactors like ports, state variables,
+actions and parameters, which are all maps from names to values of different types.
+-/
 structure Scheme where
   vars : Type
   type : vars → Type
@@ -10,6 +17,10 @@ structure Scheme where
 attribute [reducible] Scheme.type
 attribute [instance] Scheme.varsDecidableEq
 
+/--
+The (disjoint) union of two schemes describes the signature of a map where the domain is the
+disjoint union of the respective schemes' domains. The codomain is extended in the obvious way.
+-/
 abbrev Scheme.union (σ₁ σ₂ : Scheme) : Scheme where
   vars := Sum σ₁.vars σ₂.vars
   type
@@ -26,7 +37,7 @@ theorem Scheme.union_type_left (σ₁ σ₂ : Scheme) (var : σ₁.vars) :
 theorem Scheme.union_type_right (σ₁ σ₂ : Scheme) (var : σ₂.vars) :
   (σ₁ ⊎ σ₂).type (.inr var) = σ₂.type var := rfl
 
--- σs is an I-indexed family of schemes.
+/-- The big-union of schemes generalizes the notion of unions of schemes to a family of schemes. -/
 def Scheme.bUnion (σs : I → Scheme) [DecidableEq I] : Scheme where
   vars := (i : I) × (σs i).vars
   type := fun ⟨i, var⟩ => (σs i).type var
@@ -41,6 +52,15 @@ theorem Scheme.bUnion_vars (σs : I → Scheme) [DecidableEq I] :
 theorem Scheme.bUnion_type (σs : I → Scheme) [DecidableEq I] (var : (σs i).vars) :
   (⨄ σs).type ⟨i, var⟩ = (σs i).type var := rfl
 
+/--
+A scheme `σ₁` is a "subscheme" of `σ₂` if:
+1. the domain of `σ₁` is a subtype of the domain of `σ₂`, and
+2. `σ₁` and `σ₂` map the elements in `σ₁`'s domain to the same types.
+
+We express property 1 not as a `Subtype` but as the coercion `coe`. Property 2 is ensured by
+`coeEqType`. The `inv` map and additional properties provide an inverse map to `coe` (this map has
+to be partial as `coe` isn't necessarilly bijective).
+-/
 class Subscheme (σ₁ σ₂ : Scheme) where
   coe       : σ₁.vars → σ₂.vars
   inv       : σ₂.vars → Option σ₁.vars
@@ -53,44 +73,66 @@ theorem Subscheme.invEqType [inst : Subscheme σ₁ σ₂] : ∀ {b}, (inst.inv 
 
 end Interface
 
+/--
+An `Interface` over a scheme `{ vars, type }` is a map `(var : vars) → (type var)`. This type is
+used to for components in reactors like state variables and parameters, which are maps from names to
+values of different types.
+-/
 def Interface (σ : Interface.Scheme) := (var : σ.vars) → (σ.type var)
 
+/--
+An `Interface?` over a scheme `{ vars, type }` is a map `(var : vars) → Option (type var)`. This
+type is used for components in reactors like ports and actions and parameters, which are maps from
+names to values of different types which need to be able to be absent.
+-/
 def Interface? (σ : Interface.Scheme) := (var : σ.vars) → Option (σ.type var)
 
-def Interface?.empty : Interface? σ := fun _ => none
+namespace Interface?
+
+/-- The `Interface?` where every element is absent. -/
+protected def empty : Interface? σ := fun _ => none
 
 @[simp]
-theorem Interface?.empty_none : Interface?.empty var = none := rfl
+theorem empty_none : Interface?.empty var = none := rfl
 
-def Interface?.isEmpty (i : Interface? σ) := i = Interface?.empty
+/-- An `Interface?` is empty if it is `Interface?.empty` (that is, all elements are absent). -/
+def isEmpty (i : Interface? σ) := i = Interface?.empty
 
 @[simp]
-theorem Interface?.isEmpty_def (i : Interface? σ) : i.isEmpty ↔ i = Interface?.empty := by
+theorem isEmpty_def (i : Interface? σ) : i.isEmpty ↔ i = Interface?.empty := by
   simp [isEmpty]
 
-def Interface?.isPresent (i : Interface? σ) (var : σ.vars) : Bool :=
+/-- An `Interface?` is empty if it is `Interface?.empty` (that is, all elements are absent). -/
+def isPresent (i : Interface? σ) (var : σ.vars) : Bool :=
   i var |>.isSome
 
 @[simp]
-theorem Interface?.isPresent_def (i : Interface? σ) : i.isPresent var ↔ ∃ v, i var = some v := by
+theorem isPresent_def (i : Interface? σ) : i.isPresent var ↔ ∃ v, i var = some v := by
   simp [isPresent, Option.isSome_iff_exists]
 
--- Merge i₂ into i₁.
-def Interface?.merge (i₁ i₂ : Interface? σ) : Interface? σ :=
+/--
+Merges `i₂` "into" `i₁`. That is, for each element `e`:
+* if `i₁ e` is present, return that value
+* otherwise, return `i₂ e`
+-/
+def merge (i₁ i₂ : Interface? σ) : Interface? σ :=
   fun var => i₂ var |>.orElse fun _ => i₁ var
 
-theorem Interface?.merge_val₁ (i₁ i₂ : Interface? σ) : (i₂ var = none) → (i₁.merge i₂) var = i₁ var := by
+theorem merge_val₁ (i₁ i₂ : Interface? σ) : (i₂ var = none) → (i₁.merge i₂) var = i₁ var := by
   simp_all [merge, Option.orElse]
 
-theorem Interface?.merge_val₂ (i₁ i₂ : Interface? σ) : (i₂ var = some v) → (i₁.merge i₂) var = some v := by
+theorem merge_val₂ (i₁ i₂ : Interface? σ) : (i₂ var = some v) → (i₁.merge i₂) var = some v := by
   simp_all [merge, Option.orElse]
 
-theorem Interface?.merge_idem : Interface?.merge i i = i := by
+theorem merge_idem : Interface?.merge i i = i := by
   funext var
   simp [merge, Option.orElse]
   split
   · exact Eq.symm ‹_›
   · simp
 
-def Interface?.restrict [inst : Interface.Subscheme σ₁ σ₂] (i : Interface? σ₂) : Interface? σ₁ :=
+/-- Restricts the domain of the given interface to that of a given subscheme. -/
+def restrict [inst : Interface.Subscheme σ₁ σ₂] (i : Interface? σ₂) : Interface? σ₁ :=
   fun var => inst.coeEqType ▸ i (inst.coe var)
+
+end Interface?
