Runtime/Reaction/Basic.lean
@@ -2,10 +2,18 @@ import Runtime.Reaction.Monad
 
 namespace Reaction
 
-inductive Kind 
+/--
+A classifier to differentiate reactions which can use IO from those which can't. A reaction that can
+use IO is called "impure" in this context.
+-/
+inductive Kind
   | pure
   | impure
 
+/--
+Depending on a reaction's kind, its body run's in a different monad. This map associates with each
+reaction kind the monad in which the body should run.
+-/
 abbrev Kind.monad : Kind → (Type → Type)
   | pure => Id
   | impure => IO
@@ -13,6 +21,17 @@ abbrev Kind.monad : Kind → (Type → Type)
 instance {kind : Kind} : Monad kind.monad :=
   match kind with | .pure | .impure => inferInstance
 
+/--
+A reaction `Trigger` identifies an event which should cause a reaction to fire. Reactions explictly
+declare their triggers and thus the events which should cause them to fire. The different kinds of
+triggers are active under the following conditions (according to `Execution.Executable.triggers`):
+
+* `startup`: at tag (0, 0)
+* `shutdown`: at the last tag at which a given reactor system executes
+* `port p`: when the port with name `p` is present
+* `action a`: when the action with name `a` is present
+* `timer t`: when the timer with name `t` fires
+-/
 inductive Trigger (Port Action Timer : Type)
   | startup
   | shutdown
@@ -20,6 +39,14 @@ inductive Trigger (Port Action Timer : Type)
   | action (a : Action)
   | timer (t : Timer)
 
+/--
+A reaction consists chiefly of two parts:
+* a `body` which is a map from an "input context" to and "output context" (cf. `ReactionT`).
+* a list of `triggers` which determine under which conditions the reaction's body should be run.
+
+All remaining fields capture the entirety of the reaction's dependencies and are used to determine
+the exact type of the reaction's body and triggers.
+-/
 structure _root_.Reaction where
   kind          : Kind
   portSources   : Interface.Scheme
@@ -32,16 +59,22 @@ structure _root_.Reaction where
   triggers      : Array (Trigger portSources.vars actionSources.vars timers)
   body          : ReactionT portSources portEffects actionSources actionEffects state params kind.monad Unit
 
+/-- The type of the "context" passed into a reaction body upon execution. -/
 abbrev inputType (rcn : Reaction) :=
   ReactionT.Input rcn.portSources rcn.actionSources rcn.state rcn.params
 
+/-- The type of the "context" returned from a reaction body after execution. -/
 abbrev outputType (rcn : Reaction) :=
-  ReactionT.Output rcn.portEffects rcn.actionEffects rcn.state 
+  ReactionT.Output rcn.portEffects rcn.actionEffects rcn.state
 
+/-- The type of the given reaction's body. -/
 abbrev bodyType (rcn : Reaction) :=
   ReactionT rcn.portSources rcn.portEffects rcn.actionSources rcn.actionEffects rcn.state rcn.params rcn.kind.monad Unit
 
-def run (rcn : Reaction) (input : rcn.inputType) := 
+/--
+Runs a given reaction's body on a given "input context" and returns only the "output context".
+-/
+def run (rcn : Reaction) (input : rcn.inputType) :=
   Prod.fst <$> rcn.body input
 
 end Reaction
