Runtime/Utilities/README.md
@@ -1,0 +1,5 @@
+# Runtime Utilities
+
+The files in this directory are mostly transient, as they contain code which is expected to be
+part of Lean 4's `Std` or `Mathlib` at some point. As such, they are only implemented to the degree
+of being usable for execution, but contain many `sorry`s.
